experiment/Experiment.Steel.VPropList.fst
@@ -6,30 +6,32 @@ module SH = Experiment.Steel.Steel
 module Msk  = Learn.List.Mask
 
 
-let rec vprop_of_list_can_be_split (vs : vprop_list) (i : nat {i < L.length vs})
-  : Lemma (ensures can_be_split (vprop_of_list vs) (VUnit (L.index vs i))) (decreases vs)
+(***** [vprop_of_list'] *)
+
+let rec vprop_of_list'_can_be_split (vs : vprop_list) (i : nat {i < L.length vs})
+  : Lemma (ensures can_be_split (vprop_of_list' vs) (VUnit (L.index vs i))) (decreases vs)
   = let v :: vs = vs in
     if i = 0
-    then can_be_split_star_l (VUnit v) (vprop_of_list vs)
+    then can_be_split_star_l (VUnit v) (vprop_of_list' vs)
     else begin
-      can_be_split_star_r (VUnit v) (vprop_of_list vs);
-      vprop_of_list_can_be_split vs (i-1);
-      can_be_split_trans (VUnit v `star` vprop_of_list vs) (vprop_of_list vs) (VUnit (L.index vs (i-1)))
+      can_be_split_star_r (VUnit v) (vprop_of_list' vs);
+      vprop_of_list'_can_be_split vs (i-1);
+      can_be_split_trans (VUnit v `star` vprop_of_list' vs) (vprop_of_list' vs) (VUnit (L.index vs (i-1)))
     end
 
-let rec vprop_of_list_append (vs0 vs1 : vprop_list)
-  : Lemma (ensures equiv (vprop_of_list L.(vs0@vs1)) (vprop_of_list vs0 `star` vprop_of_list vs1))
+let rec vprop_of_list'_append (vs0 vs1 : vprop_list)
+  : Lemma (ensures equiv (vprop_of_list' L.(vs0@vs1)) (vprop_of_list' vs0 `star` vprop_of_list' vs1))
           (decreases vs0)
   = match vs0 with
-  | []     -> assert (equiv (vprop_of_list vs1) (emp `star` vprop_of_list vs1))
+  | []     -> assert (equiv (vprop_of_list' vs1) (emp `star` vprop_of_list' vs1))
                 by (init_resolve_tac ())
   | v :: vs -> let v0 = VUnit v in
-             let vl0 = vprop_of_list vs in
-             let vl1 = vprop_of_list vs1 in
-             let vl2 = vprop_of_list L.(vs @ vs1) in
-             assert_norm (vprop_of_list L.((v :: vs) @ vs1) == v0 `star` vl2);
+             let vl0 = vprop_of_list' vs in
+             let vl1 = vprop_of_list' vs1 in
+             let vl2 = vprop_of_list' L.(vs @ vs1) in
+             assert_norm (vprop_of_list' L.((v :: vs) @ vs1) == v0 `star` vl2);
              equiv_refl v0;
-             vprop_of_list_append vs vs1;
+             vprop_of_list'_append vs vs1;
              star_congruence v0       vl2
                              v0 (vl0 `star` vl1);
              star_associative v0 vl0 vl1;
@@ -38,7 +40,7 @@ let rec vprop_of_list_append (vs0 vs1 : vprop_list)
              equiv_trans (v0 `star` vl2)
                          (v0 `star` (vl0 `star` vl1))
                          ((v0 `star` vl0) `star` vl1);
-             assert_norm (vprop_of_list (v :: vs) `star` vprop_of_list vs1
+             assert_norm (vprop_of_list' (v :: vs) `star` vprop_of_list' vs1
                       == (v0 `star` vl0) `star` vl1)
 
 let rec flatten_vprop_aux_eq #vp ve acc
@@ -67,65 +69,101 @@ let flatten_vprop_VStar #vp0 ve0 #vp1 ve1
     flatten_vprop_aux_eq ve1 []
 
 let rec vprop_equiv_flat vp ve
-  : Lemma (ensures equiv (vprop_of_list (flatten_vprop ve)) vp) (decreases ve)
+  : Lemma (ensures equiv (vprop_of_list' (flatten_vprop ve)) vp) (decreases ve)
   = match ve with
   | VeEmp       -> equiv_refl emp
   | VeUnit v    -> assert (equiv (VUnit v `star` emp) (VUnit v))
                       by (init_resolve_tac ())
   | VeStar #vp0 ve0 #vp1 ve1 ->
            flatten_vprop_VStar ve0 ve1;
-           vprop_of_list_append (flatten_vprop ve0) (flatten_vprop ve1);
+           vprop_of_list'_append (flatten_vprop ve0) (flatten_vprop ve1);
            vprop_equiv_flat vp0 ve0;
            vprop_equiv_flat vp1 ve1;
-           star_congruence (vprop_of_list (flatten_vprop ve0)) (vprop_of_list (flatten_vprop ve1)) vp0 vp1;
-           equiv_trans (vprop_of_list L.(flatten_vprop ve0 @ flatten_vprop ve1))
-                       (vprop_of_list (flatten_vprop ve0) `star` vprop_of_list (flatten_vprop ve1))
+           star_congruence (vprop_of_list' (flatten_vprop ve0)) (vprop_of_list' (flatten_vprop ve1)) vp0 vp1;
+           equiv_trans (vprop_of_list' L.(flatten_vprop ve0 @ flatten_vprop ve1))
+                       (vprop_of_list' (flatten_vprop ve0) `star` vprop_of_list' (flatten_vprop ve1))
                        (vp0 `star` vp1)
 
+(***** [vprop_of_list] *)
 
-let sel'_sub (#p : vprop) (vs : vprop_list)
-             (h : rmem p{can_be_split p (vprop_of_list vs)})
-  : sl_t vs
-  = sel' vs (focus_rmem h (vprop_of_list vs))
+let vprop_of_list_hp (vs : vprop_list)
+  = hp_of (vprop_of_list' vs)
 
+let vprop_of_list_sel' (vs : vprop_list) : selector' (sl_f vs) (vprop_of_list_hp vs)
+  = fun (h : Mem.hmem (vprop_of_list_hp vs)) ->
+    Fl.flist_of_g (Fl.mk_flist_g (vprop_list_sels_t vs) (fun i ->
+      (**) vprop_of_list'_can_be_split vs i;
+      (**) can_be_split_interp (vprop_of_list' vs) (VUnit (L.index vs i)) h;
+      (L.index vs i).sel h
+    ))
 
-#push-options "--ifuel 1 --fuel 1"
-let rec sel_list_eq'_sub (#p : vprop) (vs : vprop_list)
-                    (h : rmem p{can_be_split p (vprop_of_list vs)})
-  : Lemma (sel_list' #p vs h == Fl.dlist_of_f_g (sel'_sub #p vs h))
-  = match vs with
-  | [] -> ()
-  | v0 :: vs ->
-       SH.rmem_star_eq (VUnit v0) (vprop_of_list vs) h;
-       calc (==) {
-         sel_list' #p (v0 :: vs) h;
-       == {}
-         Dl.DCons v0.t (h (VUnit v0)) _ (sel_list' #p vs h);
-       == { sel_list_eq'_sub #p vs h }
-         Dl.DCons v0.t (h (VUnit v0)) _ (Fl.dlist_of_f_g (sel'_sub #p vs h));
-       == { Dl.dlist_extensionality
-              (Dl.DCons v0.t (h (VUnit v0)) _ (Fl.dlist_of_f_g (sel'_sub #p vs h)))
-              (Fl.dlist_of_f_g (sel'_sub #p (v0 :: vs) h))
-              (fun i -> vprop_of_list_can_be_split (v0 :: vs) i;
-                     SH.focus_rmem_feq p (vprop_of_list (v0 :: vs)) (VUnit (L.index (v0 :: vs) i)) h;
-                     if i > 0 then begin
-                       vprop_of_list_can_be_split vs (i - 1);
-                       SH.focus_rmem_feq p (vprop_of_list vs) (VUnit (L.index vs (i - 1))) h
-                     end ) }
-         Fl.dlist_of_f_g (sel'_sub #p (v0 :: vs) h);
-       }
+#push-options "--fuel 1 --ifuel 0"
+let vprop_of_list_sel'_depends_only_on
+      (vs : vprop_list) (m0 : Mem.hmem (vprop_of_list_hp vs)) (m1 : Mem.mem {Mem.disjoint m0 m1})
+  : Lemma (vprop_of_list_sel' vs m0 == vprop_of_list_sel' vs (Mem.join m0 m1))
+  = Fl.flist_extensionality (vprop_of_list_sel' vs m0) (vprop_of_list_sel' vs (Mem.join m0 m1))
+      (fun i -> vprop_of_list'_can_be_split vs i;
+             can_be_split_interp (vprop_of_list' vs) (VUnit (L.index vs i)) m0)
+
+let vprop_of_list_sel'_depends_only_on_core
+      (vs : vprop_list) (m0 : Mem.hmem (vprop_of_list_hp vs))
+  : Lemma (vprop_of_list_sel' vs m0 == vprop_of_list_sel' vs (Mem.core_mem m0))
+  = Fl.flist_extensionality (vprop_of_list_sel' vs m0) (vprop_of_list_sel' vs (Mem.core_mem m0))
+      (fun i -> vprop_of_list'_can_be_split vs i;
+             can_be_split_interp (vprop_of_list' vs) (VUnit (L.index vs i)) m0)
 #pop-options
 
-let sel_list_eq' (vs : vprop_list) (h : rmem (vprop_of_list vs))
-  : Lemma (sel_list vs h == Fl.dlist_of_f_g (sel' vs h))
-  = sel_list_eq'_sub vs h;
-    focus_rmem_refl (vprop_of_list vs) h
+let vprop_of_list_sel (vs : vprop_list) : selector (sl_f vs) (vprop_of_list_hp vs)
+  =
+    (**) FStar.Classical.forall_intro_2 (vprop_of_list_sel'_depends_only_on      vs);
+    (**) FStar.Classical.forall_intro   (vprop_of_list_sel'_depends_only_on_core vs);
+    vprop_of_list_sel' vs
 
-let sel_eq' : squash (sel == sel_f')
-  = U.funext_eta sel_f' sel (_ by T.(trefl ())) (_ by T.(trefl ())) (fun vs ->
-    U.funext_eta_gtot (sel_f' vs) (sel vs) (_ by T.(trefl ())) (_ by T.(trefl ())) (fun h ->
-      sel_f_eq' vs h))
 
+let vprop_of_list_equiv (vs : vprop_list)
+  : Lemma (vprop_of_list vs `equiv` vprop_of_list' vs)
+  = reveal_equiv (vprop_of_list vs) (vprop_of_list' vs)
+
+let vprop_of_list_can_be_split (vs : vprop_list) (i : Ll.dom vs)
+  : Lemma (vprop_of_list vs `can_be_split` VUnit (L.index vs i))
+  = reveal_can_be_split ();
+    vprop_of_list'_can_be_split vs i
+
+let vprop_of_list_interp (vs : vprop_list) (m : Mem.mem) = ()
+let vprop_of_list_sel_eq (vs : vprop_list) (i : Ll.dom vs) (m : hmem (vprop_of_list vs)) = ()
+
+#push-options "--fuel 2 --ifuel 0 --z3rlimit 20"
+let vprop_of_list_interp_cons (v : vprop') (vs : vprop_list) (m : Mem.mem)
+  : Lemma ((Mem.interp (vprop_of_list_hp (v :: vs)) m <==> Mem.interp (v.hp `Mem.star` vprop_of_list_hp vs) m) /\
+           (Mem.interp (vprop_of_list_hp (v :: vs)) m ==>
+            vprop_of_list_sel (v :: vs) m == Fl.cons (v.sel m) (vprop_of_list_sel vs m)))
+  =
+    introduce Mem.interp (vprop_of_list_hp (v :: vs)) m ==>
+              vprop_of_list_sel (v :: vs) m == Fl.cons (v.sel m) (vprop_of_list_sel vs m)
+      with _ .
+        let lhs = vprop_of_list_sel (v :: vs) m               in
+        let rhs = Fl.cons (v.sel m) (vprop_of_list_sel vs m) in
+        Fl.flist_extensionality lhs rhs
+          (fun i ->
+            if i > 0 then begin
+              let u = L.index vs (i-1) in
+              vprop_of_list'_can_be_split vs (i-1);
+              can_be_split_interp (vprop_of_list' vs) (VUnit u) m;
+              calc (==) {
+                lhs i <: u.t;
+              == { }
+                (L.index (v :: vs) i).sel m;
+              == { }
+                u.sel m;
+              == { }
+                vprop_of_list_sel vs m (i-1);
+              == { }
+                rhs i;
+              }
+            end)
+#pop-options
+
+(*** operations *)
 
 let rew_forall_sl_f_app (v0 v1 : vprop_list) (p0 : sl_f L.(v0 @ v1) -> Type) (p1 : Type)
     (_ : squash ((forall (sl0 : sl_f v0) (sl1 : sl_f v1) . p0 (append_vars sl0 sl1)) <==> p1))
@@ -199,126 +237,116 @@ let filter_append_vars_mask
 #pop-options
 
 
-let split_vars__cons (v0 : vprop') (vs0 vs1 : vprop_list) (x0 : v0.t) (xs : sl_list L.(vs0@vs1))
-  : Lemma (ensures split_vars_list (v0 :: vs0) vs1 (Dl.DCons v0.t x0 (vprop_list_sels_t L.(vs0@vs1)) xs)
-               == (let xs0, xs1 = split_vars_list vs0 vs1 xs in
-                   Dl.DCons v0.t x0 (vprop_list_sels_t vs0) xs0, xs1))
-  = Ll.map_append Mkvprop'?.t vs0 vs1
+(**** Steel *)
 
-let steel_elim_vprop_of_list_cons_f (#opened : Mem.inames) (v : vprop') (vs : vprop_list)
-  : SteelGhost unit opened
-      (vprop_of_list (v :: vs)) (fun () -> VUnit v `star` vprop_of_list vs)
+// ALT? use steel equiv
+
+let elim_vpl_nil (#opened : Mem.inames) (vs : vprop_list {vs==[]})
+  : SteelGhost unit opened (vprop_of_list vs) (fun () -> emp)
       (requires fun _ -> True)
-      (ensures fun h0 () h1 -> sel_f (v :: vs) h0 == Fl.cons (h1 (VUnit v)) (sel_f vs h1))
+      (ensures  fun h0 _ _ -> sel_f vs h0 == Fl.nil /\ sel_list vs h0 == Dl.DNil)
   =
-    let sl0 = gget_f (v :: vs) in
-    change_equal_slprop (vprop_of_list (v :: vs)) (VUnit v `star` vprop_of_list vs);
-    let x0  = gget' v in
-    let x0  = Ghost.reveal x0 in
-    let sl1 = gget_f vs in
-    Fl.flist_extensionality sl0 (U.cast _ (Fl.cons x0 sl1)) (fun _ -> ())
+    let sl = gget_f vs in
+    Fl.nil_uniq sl;
+    rewrite_slprop (vprop_of_list vs) emp (fun m -> ())
 
-let steel_intro_vprop_of_list_cons_f (#opened : Mem.inames) (v : vprop') (vs : vprop_list)
-  : SteelGhost unit opened
-      (VUnit v `star` vprop_of_list vs) (fun () -> vprop_of_list (v :: vs))
+let intro_vpl_nil (#opened : Mem.inames) (vs : vprop_list {vs==[]})
+  : SteelGhost unit opened emp (fun () -> vprop_of_list vs)
       (requires fun _ -> True)
-      (ensures fun h0 () h1 -> sel_f (v :: vs) h1 == Fl.cons (h0 (VUnit v)) (sel_f vs h0))
+      (ensures  fun _ _ h1 -> sel_f vs h1 == Fl.nil /\ sel_list vs h1 == Dl.DNil)
   =
-    let x0  = gget' v in
-    let x0  = Ghost.reveal x0 in
-    let sl1 = gget_f vs in
-    change_equal_slprop (VUnit v `star` vprop_of_list vs) (vprop_of_list (v :: vs));
-    let sl0 = gget_f (v :: vs) in
-    Fl.flist_extensionality sl0 (U.cast _ (Fl.cons x0 sl1)) (fun _ -> ())
+    rewrite_slprop emp (vprop_of_list vs) (fun m -> ());
+    let sl = gget_f vs in
+    Fl.nil_uniq sl
+
+#push-options "--z3rlimit 50"
+let elim_vpl_cons (#opened : Mem.inames) (v : vprop') (vs : vprop_list)
+  =
+    let sl  : Ghost.erased (sl_f (v :: vs)) = gget_f (v :: vs) in
+    let sl' : Fl.flist (v.t :: vprop_list_sels_t vs) = sl in
+    change_slprop
+      (vprop_of_list (v :: vs)) (VUnit v `star` vprop_of_list vs)
+      sl (Fl.head sl', Fl.tail sl')
+      (fun m -> vprop_of_list_interp_cons v vs m;
+             assert (vprop_of_list_sel (v :: vs) m == Fl.cons (v.sel m) (vprop_of_list_sel vs m));
+             assert (v.sel m == Fl.head sl');
+             Fl.tail_cons (v.sel m) (vprop_of_list_sel vs m);
+             assert (vprop_of_list_sel vs m == Fl.tail sl'));
+    let hd = gget' v   in
+    let tl : Ghost.erased (sl_f vs) = gget_f vs in
+    Fl.as_cons sl';
+    Fl.dlist_of_f_cons (Fl.head sl') (Fl.tail sl');
+    assert (Fl.dlist_of_f sl === Dl.DCons v.t hd (vprop_list_sels_t vs) (Fl.dlist_of_f tl))
+#pop-options
+
+let intro_vpl_cons (#opened : Mem.inames) (v : vprop') (vs : vprop_list)
+  =
+    let hd = gget' v                                 in
+    let hd : v.t = Ghost.reveal hd                   in
+    let tl = gget_f vs                               in
+    let tl : sl_f vs = Ghost.reveal tl               in
+    let sl : sl_f (v :: vs) = U.cast _ (Fl.cons hd tl) in
+    change_slprop
+      (VUnit v `star` vprop_of_list vs) (vprop_of_list (v :: vs))
+      (hd, tl) sl
+      (vprop_of_list_interp_cons v vs);
+    Fl.dlist_of_f_cons hd tl
 
 
-let rec steel_elim_vprop_of_list_append #opened (vs0 vs1 : vprop_list)
+let rec elim_vpl_append_list (#opened : Mem.inames) (vs0 vs1 : vprop_list)
   : SteelGhost unit opened
       (vprop_of_list L.(vs0@vs1)) (fun () -> vprop_of_list vs0 `star` vprop_of_list vs1)
       (requires fun _ -> True)
-      (ensures fun h0 () h1 -> split_vars_list vs0 vs1 (sel_list L.(vs0@vs1) h0)
-                        == (sel_list vs0 h1, sel_list vs1 h1))
-      (decreases %[vs0; 0])
-  =
-    match vs0 with
-    | [] -> change_equal_slprop (vprop_of_list L.(vs0@vs1)) (vprop_of_list vs1);
-           change_equal_slprop emp (vprop_of_list vs0)
-    | v0 :: vs0' -> steel_elim_vprop_of_list_append__cons vs0 vs1 v0 vs0'
-
-and steel_elim_vprop_of_list_append__cons #opened (vs0 vs1 : vprop_list) v0 (vs0' : vprop_list)
-  : SteelGhost unit opened
-      (vprop_of_list L.(vs0@vs1)) (fun () -> vprop_of_list vs0 `star` vprop_of_list vs1)
-      (requires fun _ -> vs0 == v0 :: vs0')
-      (ensures fun h0 () h1 -> split_vars_list vs0 vs1 (sel_list L.(vs0@vs1) h0)
-                        == (sel_list vs0 h1, sel_list vs1 h1))
-      (decreases %[vs0'; 1])
-  =
-    change_equal_slprop (vprop_of_list L.(vs0@vs1)) (VUnit v0 `star` vprop_of_list L.(vs0'@vs1));
-    (**) let sl_v0   : Ghost.erased (v0.t) = gget' v0 in
-    (**) let sl_vs01 : Ghost.erased (t_of (vprop_of_list L.(vs0'@vs1))) = gget (vprop_of_list L.(vs0'@vs1)) in
-    steel_elim_vprop_of_list_append vs0' vs1;
-    (**) let sl_vs0  = gget (vprop_of_list vs0') in
-    (**) let sl_vs1  = gget (vprop_of_list vs1) in
-    change_equal_slprop (VUnit v0 `star` vprop_of_list vs0') (vprop_of_list (vs0));
-    calc (==) {
-      split_vars_list (v0 :: vs0') vs1 (vpl_sels L.(v0 :: vs0' @ vs1) (Ghost.reveal sl_v0, Ghost.reveal sl_vs01));
-    == {split_vars__cons v0 vs0' vs1 sl_v0 (vpl_sels L.(vs0' @ vs1) sl_vs01)}
-      (let xs0, xs1 = split_vars_list vs0' vs1 (vpl_sels L.(vs0' @ vs1) sl_vs01) in
-       Dl.DCons v0.t sl_v0 _ xs0, xs1);
-    == {}
-      Dl.DCons v0.t sl_v0 _ (vpl_sels vs0' sl_vs0), vpl_sels vs1 sl_vs1;
-    }
-
-let steel_elim_vprop_of_list_append_f #opened (vs0 vs1 : vprop_list)
-  : SteelGhost unit opened
-      (vprop_of_list L.(vs0@vs1)) (fun () -> vprop_of_list vs0 `star` vprop_of_list vs1)
-      (requires fun _ -> True)
-      (ensures fun h0 () h1 -> sel_f L.(vs0@vs1) h0 == append_vars (sel_f vs0 h1) (sel_f vs1 h1))
-  =
-    let sl = gget (vprop_of_list L.(vs0@vs1)) in
-    Ll.map_append Mkvprop'?.t vs0 vs1;
-    (* TODO: Why is this necessary ? *)
-    assert (vprop_list_sels_t L.(vs0 @ vs1) == L.(vprop_list_sels_t vs0 @ vprop_list_sels_t vs1))
-        by T.(norm [delta_only [`%vprop_list_sels_t]]; smt ());
-    Fl.splitAt_ty_of_d (vprop_list_sels_t vs0) (vprop_list_sels_t vs1) (vpl_sels L.(vs0 @ vs1) sl);
-    steel_elim_vprop_of_list_append vs0 vs1;
-    Fl.splitAt_ty_append (vprop_list_sels_t vs0) (vprop_list_sels_t vs1) (vpl_sels_f L.(vs0 @ vs1) sl)
-
-
-let rec steel_intro_vprop_of_list_append #opened (vs0 vs1 : vprop_list)
-  : SteelGhost unit opened
-      (vprop_of_list vs0 `star` vprop_of_list vs1) (fun () -> vprop_of_list L.(vs0@vs1))
-      (requires fun _ -> True)
-      (ensures fun h0 () h1 -> split_vars_list vs0 vs1 (sel_list L.(vs0@vs1) h1)
-                        == (sel_list vs0 h0, sel_list vs1 h0))
+      (ensures fun h0 () h1 ->
+         Ll.map_append Mkvprop'?.t vs0 vs1;
+         sel_list L.(vs0@vs1) h0 == Dl.append (sel_list vs0 h1) (sel_list vs1 h1))
       (decreases vs0)
   = match vs0 with
-    | [] -> change_equal_slprop (vprop_of_list vs0) emp;
-           change_equal_slprop (vprop_of_list vs1) (vprop_of_list L.(vs0@vs1))
-    | v0 :: vs0' ->
-           change_equal_slprop (vprop_of_list (vs0)) (VUnit v0 `star` vprop_of_list vs0');
-           (**) let sl_v0   = gget' v0 in
-           steel_intro_vprop_of_list_append vs0' vs1;
-           (**) let sl_vs01 = gget (vprop_of_list L.(vs0'@vs1)) in
-           (**) split_vars__cons v0 vs0' vs1 sl_v0 (vpl_sels L.(vs0' @ vs1) sl_vs01);
-           change_equal_slprop (VUnit v0 `star` vprop_of_list L.(vs0'@vs1)) (vprop_of_list L.(vs0@vs1))
+  | [] ->
+       change_equal_slprop (vprop_of_list L.(vs0@vs1)) (vprop_of_list vs1);
+       intro_vpl_nil vs0
+  | v0 :: vs0' ->
+       change_equal_slprop (vprop_of_list L.(vs0@vs1)) (vprop_of_list L.(v0 :: (vs0' @ vs1)));
+       elim_vpl_cons v0 L.(vs0' @ vs1);
+       elim_vpl_append_list vs0' vs1;
+       intro_vpl_cons v0 vs0';
+       change_equal_slprop (vprop_of_list L.(v0 :: vs0')) (vprop_of_list vs0)
 
-let steel_intro_vprop_of_list_append_f #opened (vs0 vs1 : vprop_list)
+let rec intro_vpl_append_list (#opened : Mem.inames) (vs0 vs1 : vprop_list)
   : SteelGhost unit opened
       (vprop_of_list vs0 `star` vprop_of_list vs1) (fun () -> vprop_of_list L.(vs0@vs1))
       (requires fun _ -> True)
-      (ensures fun h0 () h1 -> sel_f L.(vs0@vs1) h1 == append_vars (sel_f vs0 h0) (sel_f vs1 h0))
+      (ensures fun h0 () h1 ->
+         Ll.map_append Mkvprop'?.t vs0 vs1;
+         sel_list L.(vs0@vs1) h1 == Dl.append (sel_list vs0 h0) (sel_list vs1 h0))
+      (decreases vs0)
+  = match vs0 with
+  | [] ->
+       elim_vpl_nil vs0;
+       change_equal_slprop (vprop_of_list vs1) (vprop_of_list L.(vs0@vs1))
+  | v0 :: vs0' ->
+       change_equal_slprop (vprop_of_list vs0) (vprop_of_list L.(v0 :: vs0'));
+       elim_vpl_cons v0 vs0';
+       intro_vpl_append_list vs0' vs1;
+       intro_vpl_cons v0 L.(vs0' @ vs1);
+       change_equal_slprop (vprop_of_list L.(v0 :: (vs0' @ vs1))) (vprop_of_list L.(vs0@vs1))
+
+let elim_vpl_append #opened (vs0 vs1 : vprop_list)
   =
-    steel_intro_vprop_of_list_append vs0 vs1;
-    let sl = gget (vprop_of_list L.(vs0@vs1)) in
-    Ll.map_append Mkvprop'?.t vs0 vs1;
-    assert (vprop_list_sels_t L.(vs0 @ vs1) == L.(vprop_list_sels_t vs0 @ vprop_list_sels_t vs1))
-        by T.(norm [delta_only [`%vprop_list_sels_t]]; smt ());
-    Fl.splitAt_ty_of_d (vprop_list_sels_t vs0) (vprop_list_sels_t vs1) (vpl_sels L.(vs0 @ vs1) sl);
-    Fl.splitAt_ty_append (vprop_list_sels_t vs0) (vprop_list_sels_t vs1) (vpl_sels_f L.(vs0 @ vs1) sl)
+    elim_vpl_append_list vs0 vs1;
+    let sl0 = gget_f vs0 in
+    let sl1 = gget_f vs1 in
+    Fl.dlist_of_f_append sl0 sl1
+
+let intro_vpl_append #opened (vs0 vs1 : vprop_list)
+  =
+    let sl0 = gget_f vs0 in
+    let sl1 = gget_f vs1 in
+    intro_vpl_append_list vs0 vs1;
+    Fl.dlist_of_f_append sl0 sl1
 
 
-let rec steel_change_swap (#opened:Mem.inames)
+let rec change_vpl_swap (#opened:Mem.inames)
           (vs0 : vprop_list) (i : nat {i <= L.length vs0 - 2})
   : SteelGhost unit opened (vprop_of_list vs0) (fun () -> vprop_of_list (Perm.list_swap i vs0))
       (requires fun _ -> True) (ensures fun h0 () h1 ->
@@ -327,20 +355,22 @@ let rec steel_change_swap (#opened:Mem.inames)
   = if i = 0
     then begin
       let v0 :: v1 :: vs = vs0 in
-      change_equal_slprop (vprop_of_list vs0)
-                          (VUnit v0 `star` (VUnit v1 `star` vprop_of_list vs));
-      change_equal_slprop (VUnit v1 `star` (VUnit v0 `star` vprop_of_list vs))
-                          (vprop_of_list (Perm.list_swap i vs0))
+      change_equal_slprop (vprop_of_list vs0) (vprop_of_list (v0 :: v1 :: vs));
+      elim_vpl_cons  v0 (v1 :: vs);
+      elim_vpl_cons  v1       vs;
+      intro_vpl_cons v0       vs;
+      intro_vpl_cons v1 (v0 :: vs);
+      change_equal_slprop (vprop_of_list (v1 :: v0 :: vs)) (vprop_of_list (Perm.list_swap i vs0))
     end else begin
       let v0 :: vs = vs0 in
-      change_equal_slprop (vprop_of_list vs0)
-                          (VUnit v0 `star` vprop_of_list vs);
-      steel_change_swap vs (i-1);
-      change_equal_slprop (VUnit v0 `star` vprop_of_list (Perm.list_swap (i-1) vs))
-                          (vprop_of_list (Perm.list_swap i vs0))
+      change_equal_slprop (vprop_of_list vs0) (vprop_of_list (v0 :: vs));
+      elim_vpl_cons  v0 vs;
+      change_vpl_swap vs (i-1);
+      intro_vpl_cons v0 (Perm.list_swap (i-1) vs);
+      change_equal_slprop (vprop_of_list (v0 :: Perm.list_swap (i-1) vs)) (vprop_of_list (Perm.list_swap i vs0))
     end
 
-let rec steel_change_perm_aux (#opened:Mem.inames)
+let rec change_vpl_perm_aux (#opened:Mem.inames)
           (n : nat) (vs0 vs1 : (l:vprop_list{L.length l == n}))
           (fs : list (i:nat{i <= n-2}))
           (eqv : squash (vs1 == Perm.apply_perm_r (Perm.comp_list (L.map (Perm.perm_f_swap #n) fs)) vs0))
@@ -350,38 +380,36 @@ let rec steel_change_perm_aux (#opened:Mem.inames)
                                            (sel_list vs0 h0))
       (decreases fs)
   =
-  let sl0  = gget (vprop_of_list vs0) in
+  let sl0  = gget_list vs0 in
   match fs with
-  | []       -> change_equal_slprop (vprop_of_list vs0) (vprop_of_list vs1)
-  | f0 :: fs' -> let pfs = Perm.comp_list (L.map (Perm.perm_f_swap #n) fs') in
-               let vs' = Perm.apply_perm_r pfs vs0 in
-               steel_change_perm_aux n vs0 vs' fs' ();
-               let sl1' : sl_list vs' =
-                 Dl.apply_pequiv #(vprop_list_sels_t vs0) #(vprop_list_sels_t vs')
-                                  (vequiv_perm_sl (U.cast (Perm.perm_f (L.length vs0)) pfs))
-                                  (vpl_sels vs0 sl0) in
-               steel_change_swap vs' f0;
-               Perm.apply_swap_as_rec n f0 vs';
-               Perm.apply_r_comp (Perm.perm_f_swap #n f0) pfs vs0;
-               change_equal_slprop (vprop_of_list (Perm.list_swap f0 vs'))
-                                   (vprop_of_list vs1);
-               let sl1 = gget (vprop_of_list vs1) in
-               assert (vpl_sels vs1 sl1 === Dl.dlist_swap f0 sl1');
-               Dl.apply_swap_as_rec n f0 sl1';
-               Dl.apply_r_comp (Perm.perm_f_swap #n f0) pfs (vpl_sels vs0 sl0)
+  | [] ->
+      change_equal_slprop (vprop_of_list vs0) (vprop_of_list vs1)
+  | f0 :: fs' ->
+      let pfs = Perm.comp_list (L.map (Perm.perm_f_swap #n) fs') in
+      let vs' = Perm.apply_perm_r pfs vs0 in
+      change_vpl_perm_aux n vs0 vs' fs' ();
+      let sl1' : sl_list vs' =
+        Dl.apply_pequiv #(vprop_list_sels_t vs0) #(vprop_list_sels_t vs')
+                         (vequiv_perm_sl (U.cast (Perm.perm_f (L.length vs0)) pfs)) sl0 in
+      change_vpl_swap vs' f0;
+      Perm.apply_swap_as_rec n f0 vs';
+      Perm.apply_r_comp (Perm.perm_f_swap #n f0) pfs vs0;
+      change_equal_slprop (vprop_of_list (Perm.list_swap f0 vs'))
+                          (vprop_of_list vs1);
+      let sl1 = gget_list vs1 in
+      assert (Ghost.reveal sl1 === Dl.dlist_swap f0 sl1');
+      Dl.apply_swap_as_rec n f0 sl1';
+      Dl.apply_r_comp (Perm.perm_f_swap #n f0) pfs sl0
 
-let steel_change_perm (#vs0 #vs1 : vprop_list) (#opened:Mem.inames) (f : vequiv_perm vs0 vs1)
-  : SteelGhost unit opened (vprop_of_list vs0) (fun () -> vprop_of_list vs1)
-      (requires fun _ -> True)
-      (ensures fun h0 () h1 -> sel_f vs1 h1 == extract_vars f (sel_f vs0 h0))
+let change_vpl_perm (#vs0 #vs1 : vprop_list) (#opened:Mem.inames) (f : vequiv_perm vs0 vs1)
   =
-    let sl0 = gget (vprop_of_list vs0) in
-    Fl.apply_perm_r_of_d f (vpl_sels vs0 sl0);
-    steel_change_perm_aux (L.length vs0) vs0 vs1 (Perm.perm_f_to_swap f) ()
+    let sl0 = gget_list vs0 in
+    Fl.apply_perm_r_of_d f sl0;
+    change_vpl_perm_aux (L.length vs0) vs0 vs1 (Perm.perm_f_to_swap f) ()
 
-#push-options "--ifuel 1 --z3rlimit 20"
-// ALT? use steel equiv
-let rec elim_filter_mask #opened (vs : vprop_list) (mask : Ll.vec (L.length vs) bool)
+
+#push-options "--ifuel 1 --z3rlimit 30"
+let rec elim_vpl_filter_mask_list #opened (vs : vprop_list) (mask : Ll.vec (L.length vs) bool)
   : SteelGhost unit opened
       (vprop_of_list Msk.(filter_mask mask vs) `star`
        vprop_of_list Msk.(filter_mask (mask_not mask) vs))
@@ -393,131 +421,109 @@ let rec elim_filter_mask #opened (vs : vprop_list) (mask : Ll.vec (L.length vs) 
       (decreases vs)
   = Msk.(match mask, vs with
   | [], [] ->
-        change_equal_slprop
-           (vprop_of_list (filter_mask mask vs) `star`
-            vprop_of_list (filter_mask (Msk.mask_not mask) vs))
-           (vprop_of_list vs `star` emp)
+        change_equal_slprop (vprop_of_list (filter_mask mask vs)) (vprop_of_list vs);
+        elim_vpl_nil (filter_mask (Msk.mask_not mask) vs)
   | true  :: mask', v0 :: vs' ->
-        (**) let mask' : Ll.vec (L.length vs') bool = mask' in
-        (**) let sl1_t : Ghost.erased (t_of (vprop_of_list (filter_mask mask vs)))
-        (**)           = gget (vprop_of_list (filter_mask mask vs)) in
-        (**) let sl1_f : Ghost.erased (t_of (vprop_of_list (filter_mask (Msk.mask_not mask) vs)))
-        (**)           = gget (vprop_of_list (filter_mask (Msk.mask_not mask) vs)) in
-        change_equal_slprop (vprop_of_list (filter_mask mask vs))
-                            (VUnit v0 `star` vprop_of_list (filter_mask mask' vs'));
-        change_equal_slprop (vprop_of_list (filter_mask (Msk.mask_not mask ) vs ))
-                            (vprop_of_list (filter_mask (Msk.mask_not mask') vs'));
-        elim_filter_mask vs' mask';
-        change_equal_slprop (VUnit v0 `star` vprop_of_list vs') (vprop_of_list vs);
-        (**) let sl0 : Ghost.erased (t_of (vprop_of_list vs)) = gget (vprop_of_list vs) in
-        (**) let l0  : sl_list vs = vpl_sels vs sl0 in
-        (**) assert (vpl_sels (filter_mask mask vs) sl1_t === filter_mask_dl mask _ l0);
-        (**) assert (vpl_sels _ sl1_f === filter_mask_dl (Msk.mask_not mask) _ l0)
+        (**) let mask' : Ll.vec (L.length vs') bool = mask'         in
+        (**) let sl1_t = gget_list (filter_mask mask vs)            in
+        (**) let sl1_f = gget_list (filter_mask (mask_not mask) vs) in
+        change_equal_slprop (vprop_of_list (     filter_mask mask vs ))
+                            (vprop_of_list (v0 :: filter_mask mask' vs'));
+        change_equal_slprop (vprop_of_list (filter_mask (mask_not mask ) vs ))
+                            (vprop_of_list (filter_mask (mask_not mask') vs'));
+        elim_vpl_cons v0 (filter_mask mask' vs');
+        elim_vpl_filter_mask_list vs' mask';
+        intro_vpl_cons v0 vs';
+        change_equal_slprop (vprop_of_list (v0 :: vs')) (vprop_of_list vs);
+        (**) let sl0 = gget_list vs                                 in
+        (**) assert (Ghost.reveal sl1_t === filter_mask_dl mask _ sl0);
+        (**) assert (Ghost.reveal sl1_f === filter_mask_dl (mask_not mask) _ sl0)
   | false :: mask', v0 :: vs' ->
-        (**) let mask' : Ll.vec (L.length vs') bool = mask'           in
-        (**) let sl1_t = gget (vprop_of_list (filter_mask mask vs)) in
-        (**) let sl1_f = gget (vprop_of_list (filter_mask (Msk.mask_not mask) vs)) in
-        change_equal_slprop (vprop_of_list (filter_mask mask vs))
+        (**) let mask' : Ll.vec (L.length vs') bool = mask'         in
+        (**) let sl1_t = gget_list (filter_mask mask vs)            in
+        (**) let sl1_f = gget_list (filter_mask (mask_not mask) vs) in
+        change_equal_slprop (vprop_of_list (filter_mask mask  vs ))
                             (vprop_of_list (filter_mask mask' vs'));
-        change_equal_slprop (vprop_of_list (filter_mask (Msk.mask_not mask) vs))
-                            (VUnit v0 `star` vprop_of_list (filter_mask (Msk.mask_not mask') vs'));
-        elim_filter_mask vs' mask';
-        change_equal_slprop (VUnit v0 `star` vprop_of_list vs') (vprop_of_list vs);
-        (**) let sl0 = gget (vprop_of_list vs)        in
-        (**) let l0  : sl_list vs = vpl_sels vs sl0 in
-        (**) assert (vpl_sels _ sl1_t === filter_mask_dl mask _ l0);
-        (**) assert (vpl_sels _ sl1_f === filter_mask_dl (Msk.mask_not mask) _ l0)
+        change_equal_slprop (vprop_of_list (    filter_mask (mask_not mask ) vs ))
+                            (vprop_of_list (v0 :: filter_mask (mask_not mask') vs'));
+        elim_vpl_cons v0 (filter_mask (mask_not mask') vs');
+        elim_vpl_filter_mask_list vs' mask';
+        intro_vpl_cons v0 vs';
+        change_equal_slprop (vprop_of_list (v0 :: vs')) (vprop_of_list vs);
+        (**) let sl0 = gget_list vs                                 in
+        (**) assert (Ghost.reveal sl1_t === filter_mask_dl mask _ sl0);
+        (**) assert (Ghost.reveal sl1_f === filter_mask_dl (Msk.mask_not mask) _ sl0)
   )
 
-let rec intro_filter_mask #opened (vs : vprop_list) (mask : Ll.vec (L.length vs) bool)
+let rec intro_vpl_filter_mask_list #opened (vs : vprop_list) (mask : Ll.vec (L.length vs) bool)
   : SteelGhost unit opened
       (vprop_of_list vs)
       (fun () -> vprop_of_list Msk.(filter_mask mask vs) `star`
               vprop_of_list Msk.(filter_mask (mask_not mask) vs))
       (requires fun _ -> True) Msk.(ensures fun h0 () h1 ->
           sel_list (filter_mask mask vs) h1 == filter_mask_dl mask _ (sel_list vs h0) /\
-          sel_list (filter_mask (Msk.mask_not mask) vs) h1 ==
-            filter_mask_dl (Msk.mask_not mask) _ (sel_list vs h0))
+          sel_list (filter_mask (mask_not mask) vs) h1 ==
+            filter_mask_dl (mask_not mask) _ (sel_list vs h0))
       (decreases vs)
   = Msk.(match mask, vs with
   | [], [] ->
-        change_equal_slprop
-           (vprop_of_list vs `star` emp)
-           (vprop_of_list (filter_mask mask vs) `star`
-            vprop_of_list (filter_mask (Msk.mask_not mask) vs))
+        intro_vpl_nil (filter_mask (Msk.mask_not mask) vs);
+        change_equal_slprop (vprop_of_list vs) (vprop_of_list (filter_mask mask vs))
   | true  :: mask', v0 :: vs' ->
-        (**) let mask' : Ll.vec (L.length vs') bool = mask' in
-        (**) let sl0 : Ghost.erased (t_of (vprop_of_list vs)) = gget (vprop_of_list vs) in
-        (**) let l0  : sl_list vs = vpl_sels vs sl0 in
-        change_equal_slprop (vprop_of_list vs) (VUnit v0 `star` vprop_of_list vs');
-        intro_filter_mask vs' mask';
-        change_equal_slprop (VUnit v0 `star` vprop_of_list (filter_mask mask' vs'))
-                            (vprop_of_list (filter_mask mask vs));
-        change_equal_slprop (vprop_of_list (filter_mask (Msk.mask_not mask') vs'))
-                            (vprop_of_list (filter_mask (Msk.mask_not mask ) vs ));
-        (**) let sl1_t : Ghost.erased (t_of (vprop_of_list (filter_mask mask vs)))
-        (**)           = gget (vprop_of_list (filter_mask mask vs)) in
-        (**) let sl1_f : Ghost.erased (t_of (vprop_of_list (filter_mask (Msk.mask_not mask) vs)))
-        (**)           = gget (vprop_of_list (filter_mask (Msk.mask_not mask) vs)) in
-        (**) let l1_t  : sl_list (filter_mask mask vs) = vpl_sels (filter_mask mask vs) sl1_t in
-        (**) let l1_t' : sl_list (filter_mask mask vs) = U.cast _ (filter_mask_dl mask _ l0) in
-        (**) assert (l1_t == l1_t');
-        (**) assert (vpl_sels _ sl1_f === filter_mask_dl (Msk.mask_not mask) _ l0)
+        (**) let mask' : Ll.vec (L.length vs') bool = mask'         in
+        (**) let sl0 = gget_list vs                                 in
+        change_equal_slprop (vprop_of_list vs) (vprop_of_list (v0 :: vs'));
+        elim_vpl_cons v0 vs';
+        intro_vpl_filter_mask_list vs' mask';
+        intro_vpl_cons v0 (filter_mask mask' vs');
+        change_equal_slprop (vprop_of_list (v0 :: filter_mask mask' vs'))
+                            (vprop_of_list (     filter_mask mask vs ));
+        change_equal_slprop (vprop_of_list (filter_mask (mask_not mask') vs'))
+                            (vprop_of_list (filter_mask (mask_not mask ) vs ));
+        (**) let sl1_t = gget_list (filter_mask mask vs)            in
+        (**) let sl1_f = gget_list (filter_mask (mask_not mask) vs) in
+        (**) assert (Ghost.reveal sl1_t === filter_mask_dl mask _ sl0);
+        (**) assert (Ghost.reveal sl1_f === filter_mask_dl (mask_not mask) _ sl0)
   | false :: mask', v0 :: vs' ->
-        (**) let mask' : Ll.vec (L.length vs') bool = mask' in
-        (**) let sl0 = gget (vprop_of_list vs)            in
-        (**) let l0  : sl_list vs = vpl_sels vs sl0     in
-        change_equal_slprop (vprop_of_list vs) (VUnit v0 `star` vprop_of_list vs');
-        intro_filter_mask vs' mask';
+        (**) let mask' : Ll.vec (L.length vs') bool = mask'         in
+        (**) let sl0 = gget_list vs                                 in
+        change_equal_slprop (vprop_of_list vs) (vprop_of_list (v0 :: vs'));
+        elim_vpl_cons v0 vs';
+        intro_vpl_filter_mask_list vs' mask';
+        intro_vpl_cons v0 (filter_mask (mask_not mask') vs');
         change_equal_slprop (vprop_of_list (filter_mask mask' vs'))
-                            (vprop_of_list (filter_mask mask vs));
-        change_equal_slprop (VUnit v0 `star` vprop_of_list (filter_mask (Msk.mask_not mask') vs'))
-                            (vprop_of_list (filter_mask (Msk.mask_not mask) vs));
-        (**) let sl1_t = gget (vprop_of_list (filter_mask mask vs))                in
-        (**) let sl1_f = gget (vprop_of_list (filter_mask (Msk.mask_not mask) vs)) in
-        (**) assert (vpl_sels _ sl1_t === filter_mask_dl mask _ l0);
-        (**) assert (vpl_sels _ sl1_f === filter_mask_dl (Msk.mask_not mask) _ l0)
+                            (vprop_of_list (filter_mask mask  vs ));
+        change_equal_slprop (vprop_of_list (v0 :: filter_mask (mask_not mask') vs'))
+                            (vprop_of_list (    filter_mask (mask_not mask ) vs ));
+        (**) let sl1_t = gget_list (filter_mask mask vs)            in
+        (**) let sl1_f = gget_list (filter_mask (mask_not mask) vs) in
+        (**) assert (Ghost.reveal sl1_t === filter_mask_dl mask _ sl0);
+        (**) assert (Ghost.reveal sl1_f === filter_mask_dl (Msk.mask_not mask) _ sl0)
   )
 #pop-options
 
-
-let intro_elim_filter_mask_append_lem
-      (vs : vprop_list) (m : Ll.vec (L.length vs) bool)
-      (sl : sl_list vs) (sl0 : sl_list Msk.(filter_mask m vs)) (sl1 : sl_list Msk.(filter_mask (mask_not m) vs))
-  : Lemma (requires sl0 == Msk.filter_mask_dl m _ sl /\ sl1 == Msk.filter_mask_dl (Msk.mask_not m) _ sl)
-          (ensures  Fl.flist_of_d sl == append_vars_mask m (Fl.flist_of_d sl0) (Fl.flist_of_d sl1))
+let elim_vpl_filter_mask (#opened : Mem.inames) (vs : vprop_list) (mask : Ll.vec (L.length vs) bool)
   =
-    Msk.filter_mask_f_dl_f m _ (Fl.flist_of_d sl);
-    assert (Fl.flist_of_d sl0 == Msk.filter_mask_fl m _ (Fl.flist_of_d sl));
-    Msk.filter_mask_f_dl_f (Msk.mask_not m) _ (Fl.flist_of_d sl);
-    append_filter_vars_mask m (Fl.flist_of_d sl)
+    elim_vpl_filter_mask_list vs mask;
+    let sl = gget_f vs in
+    Msk.filter_mask_f_dl_f mask _ sl;
+    Msk.filter_mask_f_dl_f (Msk.mask_not mask) _ sl
 
-let elim_filter_mask_append (#opened : Mem.inames) (vs : vprop_list) (m : Ll.vec (L.length vs) bool)
-  : SteelGhost unit opened
-      (vprop_of_list Msk.(filter_mask           m  vs) `star` 
-       vprop_of_list Msk.(filter_mask (mask_not m) vs))
-      (fun () -> vprop_of_list vs)
-      (requires fun _ -> True) (ensures fun h0 () h1 ->
-          sel_f vs h1 == append_vars_mask m (sel_f Msk.(filter_mask m vs) h0)
-                                            (sel_f Msk.(filter_mask (mask_not m) vs) h0))
+let intro_vpl_filter_mask (#opened : Mem.inames) (vs : vprop_list) (mask : Ll.vec (L.length vs) bool)
   =
-    let sl0 = gget (vprop_of_list Msk.(filter_mask           m  vs)) in
-    let sl1 = gget (vprop_of_list Msk.(filter_mask (mask_not m) vs)) in
-    elim_filter_mask vs m;
-    let sl  = gget (vprop_of_list vs)                                in
-    intro_elim_filter_mask_append_lem vs m (vpl_sels _ sl) (vpl_sels _ sl0) (vpl_sels _ sl1)
+    let sl = gget_f vs in
+    intro_vpl_filter_mask_list vs mask;
+    Msk.filter_mask_f_dl_f mask _ sl;
+    Msk.filter_mask_f_dl_f (Msk.mask_not mask) _ sl
 
-let intro_filter_mask_append (#opened : Mem.inames) (vs : vprop_list) (m : Ll.vec (L.length vs) bool)
-  : SteelGhost unit opened
-      (vprop_of_list vs)
-      (fun () -> vprop_of_list Msk.(filter_mask           m  vs) `star` 
-              vprop_of_list Msk.(filter_mask (mask_not m) vs))
-      (requires fun _ -> True) (ensures fun h0 () h1 ->
-          sel_f vs h0 == append_vars_mask m (sel_f Msk.(filter_mask m vs) h1)
-                                            (sel_f Msk.(filter_mask (mask_not m) vs) h1))
+let elim_vpl_filter_mask_append (#opened : Mem.inames) (vs : vprop_list) (m : Ll.vec (L.length vs) bool)
   =
-    let sl  = gget (vprop_of_list vs)                                in
-    intro_filter_mask vs m;
-    let sl0 = gget (vprop_of_list Msk.(filter_mask           m  vs)) in
-    let sl1 = gget (vprop_of_list Msk.(filter_mask (mask_not m) vs)) in
-    intro_elim_filter_mask_append_lem vs m (vpl_sels _ sl) (vpl_sels _ sl0) (vpl_sels _ sl1)
+    elim_vpl_filter_mask vs m;
+    let sl  = gget_f vs in
+    append_filter_vars_mask m sl
+
+let intro_vpl_filter_mask_append (#opened : Mem.inames) (vs : vprop_list) (m : Ll.vec (L.length vs) bool)
+  =
+    let sl  = gget_f vs in
+    intro_vpl_filter_mask vs m;
+    append_filter_vars_mask m sl
