experiment/Experiment.Steel.VPropList.fsti
@@ -14,19 +14,19 @@ open Steel.Effect.Atomic
 
 type vprop_list = list vprop'
 
+(***** [vprop_of_list'] *)
+
 [@@ __reduce__]
 let rec vprop_of_list' (vpl : vprop_list) : vprop =
   match vpl with
   | [] -> emp
   | v :: vs -> VStar (VUnit v) (vprop_of_list' vs)
 
-let vprop_of_list = vprop_of_list'
+val vprop_of_list'_can_be_split (vs : vprop_list) (i : nat {i < L.length vs})
+  : Lemma (can_be_split (vprop_of_list' vs) (VUnit (L.index vs i)))
 
-val vprop_of_list_can_be_split (vs : vprop_list) (i : nat {i < L.length vs})
-  : Lemma (can_be_split (vprop_of_list vs) (VUnit (L.index vs i)))
-
-val vprop_of_list_append (vs0 vs1 : vprop_list)
-  : Lemma (equiv (vprop_of_list L.(vs0@vs1)) (vprop_of_list vs0 `star` vprop_of_list vs1))
+val vprop_of_list'_append (vs0 vs1 : vprop_list)
+  : Lemma (equiv (vprop_of_list' L.(vs0@vs1)) (vprop_of_list' vs0 `star` vprop_of_list' vs1))
 
 
 noeq
@@ -52,24 +52,22 @@ val flatten_vprop_VStar (#vp0 : vprop) (ve0 : vprop_with_emp vp0) (#vp1 : vprop)
   : Lemma (flatten_vprop (VeStar ve0 ve1) == L.(flatten_vprop ve0 @ flatten_vprop ve1))
 
 val vprop_equiv_flat (vp : vprop) (ve : vprop_with_emp vp)
-  : Lemma (equiv (vprop_of_list (flatten_vprop ve)) vp)
+  : Lemma (equiv (vprop_of_list' (flatten_vprop ve)) vp)
 
 
 noeq
 type vprop_to_list (v : vprop) : (vs : vprop_list) -> Type =
   | VPropToList : (ve : vprop_with_emp v) -> vprop_to_list v (flatten_vprop ve)
 
-let vprop_to_list_equiv (#v : vprop) (#vs : vprop_list) (t : vprop_to_list v vs)
-  : Lemma (v `equiv` vprop_of_list vs)
+let vprop_to_list_equiv' (#v : vprop) (#vs : vprop_list) (t : vprop_to_list v vs)
+  : Lemma (v `equiv` vprop_of_list' vs)
   =
     let VPropToList ve = t in
     vprop_equiv_flat v ve;
-    equiv_sym (vprop_of_list vs) v
+    equiv_sym (vprop_of_list' vs) v
 
 
 (***** selectors *)
-
-(* ALT? dependent arrrow Fin.fin n -> _ *)
 
 let vprop_list_sels_t : vprop_list -> Dl.ty_list =
   L.map Mkvprop'?.t
@@ -88,77 +86,86 @@ let vprop_list_sels_t_eq (vs : vprop_list) (i : nat {i < L.length vs})
           [SMTPat (L.index (vprop_list_sels_t vs) i)]
   = Ll.map_index Mkvprop'?.t vs i
 
-let rec vpl_sels (vs : vprop_list) (sl : t_of (vprop_of_list vs))
-  : Tot (sl_list vs) (decreases vs)
-  = match (|vs, sl|) <: (vs : vprop_list & t_of (vprop_of_list vs)) with
-  | (|[], _|) -> Dl.DNil
-  | (|v0 :: vs, sl|) -> Dl.DCons v0.t sl._1 _ (vpl_sels vs sl._2)
 
-unfold
-let vpl_sels_f (vs : vprop_list) (sl : t_of (vprop_of_list vs)) : sl_f vs
-  = Fl.flist_of_d (vpl_sels vs sl)
+(***** [vprop_of_list] *)
 
-unfold
-let sel_list' (#p : vprop) (vs : vprop_list)
-      (h : rmem p{can_be_split p (vprop_of_list vs)})
-  : GTot (sl_list vs)
-  = vpl_sels vs (h (vprop_of_list vs))
+// We cannot use [sl_list vs] as selector type since it is in universe u#1, be [sl_f vs] works
 
-unfold
-let sel_list (#p : vprop) (vs : vprop_list)
-      (h : rmem p{FStar.Tactics.with_tactic selector_tactic (can_be_split p (vprop_of_list vs) /\ True)})
-  : GTot (sl_list vs)
-  = sel_list' vs h
+val vprop_of_list_hp  (vs : vprop_list) : Mem.slprop u#1
+
+val vprop_of_list_sel (vs : vprop_list) : selector (sl_f vs) (vprop_of_list_hp vs)
+
+[@@__steel_reduce__]
+let vprop_of_list_r (vs : vprop_list) : vprop' =
+  {
+    hp  = vprop_of_list_hp vs;
+    t   = sl_f vs;
+    sel = vprop_of_list_sel vs;
+  }
+unfold let vprop_of_list (vs : vprop_list) : vprop =
+  VUnit (vprop_of_list_r vs)
+
+val vprop_of_list_equiv (vs : vprop_list)
+  : Lemma (vprop_of_list vs `equiv` vprop_of_list' vs)
+
+val vprop_of_list_can_be_split (vs : vprop_list) (i : Ll.dom vs)
+  : Lemma (vprop_of_list vs `can_be_split` VUnit (L.index vs i))
+
+val vprop_of_list_interp (vs : vprop_list) (m : Mem.mem)
+  : Lemma (Mem.interp (vprop_of_list_hp vs) m <==> Mem.interp (hp_of (vprop_of_list' vs)) m)
+
+val vprop_of_list_sel_eq (vs : vprop_list) (i : Ll.dom vs) (m : hmem (vprop_of_list vs))
+  : Lemma (
+      (**) vprop_of_list_can_be_split vs i;
+      (**) can_be_split_interp (vprop_of_list vs) (VUnit (L.index vs i)) m;
+      vprop_of_list_sel vs m i == (L.index vs i).sel m)
+
+val vprop_of_list_interp_cons (v : vprop') (vs : vprop_list) (m : Mem.mem)
+  : Lemma ((Mem.interp (vprop_of_list_hp (v :: vs)) m <==> Mem.interp (v.hp `Mem.star` vprop_of_list_hp vs) m) /\
+           (Mem.interp (vprop_of_list_hp (v :: vs)) m ==>
+            vprop_of_list_sel (v :: vs) m == Fl.cons (v.sel m) (vprop_of_list_sel vs m)))
+
+let vprop_to_list_equiv (#v : vprop) (#vs : vprop_list) (t : vprop_to_list v vs)
+  : Lemma (v `equiv` vprop_of_list vs)
+  =
+    vprop_to_list_equiv' t;
+    vprop_of_list_equiv vs;
+    equiv_sym (vprop_of_list vs) (vprop_of_list' vs);
+    equiv_trans v (vprop_of_list' vs) (vprop_of_list vs)
 
 unfold
 let sel_f (#p : vprop) (vs : vprop_list)
       (h : rmem p{FStar.Tactics.with_tactic selector_tactic (can_be_split p (vprop_of_list vs) /\ True)})
   : GTot (sl_f vs)
-  = Fl.flist_of_d (sel_list vs h)
+  = h (vprop_of_list vs)
 
 unfold
-let sel (vs : vprop_list) (h : rmem (vprop_of_list vs))
-  : GTot (sl_f vs)
-  = sel_f vs h
-
-
-/// Variant to be used when interacting with Steel
-let sel' (vs : vprop_list) (h : rmem (vprop_of_list' vs))
-  : sl_t vs
-  = Fl.mk_flist_g (vprop_list_sels_t vs) (fun i ->
-    (**) vprop_of_list_can_be_split vs i;
-    h (VUnit (L.index vs i)))
-
-let sel_f' (vs : vprop_list) (h : rmem (vprop_of_list' vs))
-  : GTot (sl_f vs)
-  = Fl.flist_of_g (sel' vs h)
-
-val sel_list_eq' (vs : vprop_list) (h : rmem (vprop_of_list vs))
-  : Lemma (sel_list vs h == Fl.dlist_of_f_g (sel' vs h))
-
-let sel_f_eq' (vs : vprop_list) (h : rmem (vprop_of_list vs))
-  : Lemma (sel_f vs h == sel_f' vs h)
-  = sel_list_eq' vs h
-
-val sel_eq' : squash (sel_f' == sel)
+let sel_list (#p : vprop) (vs : vprop_list)
+      (h : rmem p{FStar.Tactics.with_tactic selector_tactic (can_be_split p (vprop_of_list vs) /\ True)})
+  : GTot (sl_list vs)
+  = Fl.dlist_of_f (h (vprop_of_list vs))
 
 
 let gget' (#opened : Mem.inames) (p : vprop')
   : SteelGhost (Ghost.erased p.t) opened (VUnit p) (fun _ -> VUnit p)
-               (requires fun _ -> True)
-               (ensures fun h0 x h1 -> frame_equalities (VUnit p) h0 h1 /\ Ghost.reveal x == h0 (VUnit p))
+      (requires fun _ -> True)
+      (ensures  fun h0 x h1 -> frame_equalities (VUnit p) h0 h1 /\ Ghost.reveal x == h0 (VUnit p))
   = gget (VUnit p)
 
 let gget_f (#opened : Mem.inames) (vs : vprop_list)
   : SteelGhost (Ghost.erased (sl_f vs)) opened (vprop_of_list vs) (fun _ -> vprop_of_list vs)
-               (requires fun _ -> True)
-               (ensures fun h0 x h1 -> frame_equalities (vprop_of_list vs) h0 h1 /\
-                                    Ghost.reveal x == sel_f vs h0)
-  = let x = gget (vprop_of_list vs) in
-    vpl_sels_f vs x
+      (requires fun _ -> True)
+      (ensures  fun h0 sl h1 -> frame_equalities (vprop_of_list vs) h0 h1 /\ Ghost.reveal sl == sel_f vs h0)
+  = gget (vprop_of_list vs)
 
+let gget_list (#opened : Mem.inames) (vs : vprop_list)
+  : SteelGhost (Ghost.erased (sl_list vs)) opened (vprop_of_list vs) (fun _ -> vprop_of_list vs)
+      (requires fun _ -> True)
+      (ensures  fun h0 sl h1 -> frame_equalities (vprop_of_list vs) h0 h1 /\ Ghost.reveal sl == sel_list vs h0)
+  = let sl = gget (vprop_of_list vs) in
+    Fl.dlist_of_f sl
 
-(***** operations *)
+(*** operations *)
 
 unfold
 let split_vars (vs0 vs1 : vprop_list) (xs : sl_f L.(vs0 @ vs1))
@@ -278,60 +285,74 @@ val filter_append_vars_mask
            filter_sl (Msk.mask_not m) (append_vars_mask m sl0 sl1) == sl1)
 
 
-val steel_elim_vprop_of_list_cons_f (#opened : Mem.inames) (v : vprop') (vs : vprop_list)
+(**** Steel *)
+
+val elim_vpl_nil (#opened : Mem.inames) (vs : vprop_list {vs==[]})
+  : SteelGhost unit opened (vprop_of_list vs) (fun () -> emp)
+      (requires fun _ -> True)
+      (ensures  fun h0 _ _ -> sel_f    vs h0 == Fl.nil /\
+                           sel_list vs h0 == Dl.DNil)
+
+val intro_vpl_nil (#opened : Mem.inames) (vs : vprop_list {vs==[]})
+  : SteelGhost unit opened emp (fun () -> vprop_of_list vs)
+      (requires fun _ -> True)
+      (ensures  fun _ _ h1 -> sel_f    vs h1 == Fl.nil /\
+                           sel_list vs h1 == Dl.DNil)
+
+val elim_vpl_cons (#opened : Mem.inames) (v : vprop') (vs : vprop_list)
   : SteelGhost unit opened
       (vprop_of_list (v :: vs)) (fun () -> VUnit v `star` vprop_of_list vs)
       (requires fun _ -> True)
-      (ensures fun h0 () h1 -> sel_f (v :: vs) h0 == Fl.cons (h1 (VUnit v)) (sel_f vs h1))
+      (ensures fun h0 () h1 -> sel_f    (v :: vs) h0 == Fl.cons    (h1 (VUnit v))   (sel_f    vs h1) /\
+                            sel_list (v :: vs) h0 == Dl.DCons _ (h1 (VUnit v)) _ (sel_list vs h1))
 
-val steel_intro_vprop_of_list_cons_f (#opened : Mem.inames) (v : vprop') (vs : vprop_list)
+val intro_vpl_cons (#opened : Mem.inames) (v : vprop') (vs : vprop_list)
   : SteelGhost unit opened
       (VUnit v `star` vprop_of_list vs) (fun () -> vprop_of_list (v :: vs))
       (requires fun _ -> True)
-      (ensures fun h0 () h1 -> sel_f (v :: vs) h1 == Fl.cons (h0 (VUnit v)) (sel_f vs h0))
+      (ensures fun h0 () h1 -> sel_f    (v :: vs) h1 == Fl.cons    (h0 (VUnit v))   (sel_f    vs h0) /\
+                            sel_list (v :: vs) h1 == Dl.DCons _ (h0 (VUnit v)) _ (sel_list vs h0))
 
 
-val steel_elim_vprop_of_list_append_f (#opened : Mem.inames) (vs0 vs1 : vprop_list)
+val elim_vpl_append (#opened : Mem.inames) (vs0 vs1 : vprop_list)
   : SteelGhost unit opened
       (vprop_of_list L.(vs0@vs1)) (fun () -> vprop_of_list vs0 `star` vprop_of_list vs1)
       (requires fun _ -> True)
       (ensures fun h0 () h1 -> sel_f L.(vs0@vs1) h0 == append_vars (sel_f vs0 h1) (sel_f vs1 h1))
 
-val steel_intro_vprop_of_list_append_f (#opened : Mem.inames) (vs0 vs1 : vprop_list)
+val intro_vpl_append (#opened : Mem.inames) (vs0 vs1 : vprop_list)
   : SteelGhost unit opened
       (vprop_of_list vs0 `star` vprop_of_list vs1) (fun () -> vprop_of_list L.(vs0@vs1))
       (requires fun _ -> True)
       (ensures fun h0 () h1 -> sel_f L.(vs0@vs1) h1 == append_vars (sel_f vs0 h0) (sel_f vs1 h0))
 
 
-val steel_change_perm (#vs0 #vs1 : vprop_list) (#opened:Mem.inames) (f : vequiv_perm vs0 vs1)
+val change_vpl_perm (#vs0 #vs1 : vprop_list) (#opened:Mem.inames) (f : vequiv_perm vs0 vs1)
   : SteelGhost unit opened (vprop_of_list vs0) (fun () -> vprop_of_list vs1)
       (requires fun _ -> True)
       (ensures fun h0 () h1 -> sel_f vs1 h1 == extract_vars f (sel_f vs0 h0))
 
 
-val elim_filter_mask (#opened : Mem.inames) (vs : vprop_list) (mask : Ll.vec (L.length vs) bool)
+val elim_vpl_filter_mask (#opened : Mem.inames) (vs : vprop_list) (mask : Ll.vec (L.length vs) bool)
   : SteelGhost unit opened
       (vprop_of_list Msk.(filter_mask mask vs) `star`
        vprop_of_list Msk.(filter_mask (mask_not mask) vs))
       (fun () -> vprop_of_list vs)
       (requires fun _ -> True) (ensures fun h0 () h1 ->
-          sel_list Msk.(filter_mask mask vs) h0 == Msk.filter_mask_dl mask _ (sel_list vs h1) /\
-          sel_list Msk.(filter_mask (mask_not mask) vs) h0 ==
-            Msk.filter_mask_dl (Msk.mask_not mask) _ (sel_list vs h1))
+          sel_f Msk.(filter_mask mask vs) h0 == filter_sl mask (sel_f vs h1) /\
+          sel_f Msk.(filter_mask (mask_not mask) vs) h0 == filter_sl (Msk.mask_not mask) (sel_f vs h1))
 
-val intro_filter_mask (#opened : Mem.inames) (vs : vprop_list) (mask : Ll.vec (L.length vs) bool)
+val intro_vpl_filter_mask (#opened : Mem.inames) (vs : vprop_list) (mask : Ll.vec (L.length vs) bool)
   : SteelGhost unit opened
       (vprop_of_list vs)
       (fun () -> vprop_of_list Msk.(filter_mask mask vs) `star`
               vprop_of_list Msk.(filter_mask (mask_not mask) vs))
       (requires fun _ -> True) (ensures fun h0 () h1 ->
-          sel_list Msk.(filter_mask mask vs) h1 == Msk.filter_mask_dl mask _ (sel_list vs h0) /\
-          sel_list Msk.(filter_mask (mask_not mask) vs) h1 ==
-            Msk.filter_mask_dl (Msk.mask_not mask) _ (sel_list vs h0))
+          sel_f Msk.(filter_mask mask vs) h1 == filter_sl mask (sel_f vs h0) /\
+          sel_f Msk.(filter_mask (mask_not mask) vs) h1 == filter_sl (Msk.mask_not mask) (sel_f vs h0))
 
 
-val elim_filter_mask_append (#opened : Mem.inames) (vs : vprop_list) (m : Ll.vec (L.length vs) bool)
+val elim_vpl_filter_mask_append (#opened : Mem.inames) (vs : vprop_list) (m : Ll.vec (L.length vs) bool)
   : SteelGhost unit opened
       (vprop_of_list Msk.(filter_mask           m  vs) `star` 
        vprop_of_list Msk.(filter_mask (mask_not m) vs))
@@ -340,7 +361,7 @@ val elim_filter_mask_append (#opened : Mem.inames) (vs : vprop_list) (m : Ll.vec
           sel_f vs h1 == append_vars_mask m (sel_f Msk.(filter_mask m vs) h0)
                                             (sel_f Msk.(filter_mask (mask_not m) vs) h0))
 
-val intro_filter_mask_append (#opened : Mem.inames) (vs : vprop_list) (m : Ll.vec (L.length vs) bool)
+val intro_vpl_filter_mask_append (#opened : Mem.inames) (vs : vprop_list) (m : Ll.vec (L.length vs) bool)
   : SteelGhost unit opened
       (vprop_of_list vs)
       (fun () -> vprop_of_list Msk.(filter_mask           m  vs) `star` 
