experiment/Experiment.Steel.Repr.M.fst
@@ -7,17 +7,6 @@ module L = FStar.List.Pure
 
 (*** [repr_steel_t] *)
 
-let steel_of_repr_lem #a #pre #post #req #ens (tr : to_repr_t a pre post req ens)
-  : Lemma (pre `equiv` vprop_of_list tr.r_pre /\
-           pre `can_be_split` vprop_of_list tr.r_pre /\
-           (forall (x : a) . can_be_split (post x) (vprop_of_list (tr.r_post x))))
-  =
-    tr.r_pre_eq ();
-    equiv_can_be_split pre (vprop_of_list tr.r_pre);
-    introduce forall (x : a) . can_be_split (post x) (vprop_of_list (tr.r_post x))
-      with (tr.r_post_eq x;
-            equiv_can_be_split (post x) (vprop_of_list (tr.r_post x)))
-
 inline_for_extraction noextract
 let steel_of_repr
       (#a : Type) (#pre : SE.pre_t) (#post : SE.post_t a) (#req : SE.req_t pre) (#ens : SE.ens_t pre a post)
@@ -25,22 +14,16 @@ let steel_of_repr
       (f : repr_steel_t SH.KSteel a tr.r_pre tr.r_post tr.r_req tr.r_ens)
   : SH.unit_steel a pre post req ens
   =
-    (**) steel_of_repr_lem tr;
-    (**) FStar.Classical.forall_intro tr.r_req_eq;
-    (**) FStar.Classical.forall_intro_3 tr.r_ens_eq;
+    (**) tr.r_pre_eq ();
+    (**) FStar.Classical.forall_intro tr.r_post_eq;
+    (**) FStar.Classical.forall_intro_2 reveal_equiv;
     SH.unit_steel_subcomp_no_frame
       _ _ req ens
       (tr.r_pre_eq ()) (fun x -> tr.r_post_eq x)
-      ()
+      (SH.intro_subcomp_no_frame_pre _ _ _ _ _ _
+        (fun h0      -> tr.r_req_eq h0)
+        (fun h0 x h1 -> tr.r_ens_eq h0 x h1))
       (SH.steel_u f)
-
-let repr_steel_of_steel_lem #a #pre #post #req #ens (tr : to_repr_t a pre post req ens)
-  : Lemma (vprop_of_list tr.r_pre `equiv` pre /\
-           (forall (x : a) . vprop_of_list (tr.r_post x) `equiv` post x))
-  =
-    tr.r_pre_eq (); equiv_sym pre (vprop_of_list tr.r_pre);
-    introduce forall (x : a) . vprop_of_list (tr.r_post x) `equiv` post x
-      with (tr.r_post_eq x; equiv_sym (post x) (vprop_of_list (tr.r_post x)))
 
 inline_for_extraction noextract
 let repr_steel_of_steel
@@ -49,16 +32,17 @@ let repr_steel_of_steel
       ($f  : SH.unit_steel a pre post req ens)
   : repr_steel_t SH.KSteel a tr.r_pre tr.r_post tr.r_req tr.r_ens
   =
-    (**) steel_of_repr_lem tr;
-    (**) repr_steel_of_steel_lem tr;
-    (**) FStar.Classical.forall_intro tr.r_req_eq;
-    (**) FStar.Classical.forall_intro_3 tr.r_ens_eq;
+    (**) tr.r_pre_eq ();
+    (**) FStar.Classical.forall_intro tr.r_post_eq;
+    (**) FStar.Classical.forall_intro_2 reveal_equiv;
     SH.steel_f (SH.unit_steel_subcomp_no_frame
       req ens _ _
       () (fun _ -> ())
       (SH.intro_subcomp_no_frame_pre _ _ _ _ _ _
-        (fun h0 -> tr.r_req_eq (focus_rmem h0 pre))
-        (fun h0 x h1 -> tr.r_ens_eq (focus_rmem h0 pre) x (focus_rmem h1 (post x))))
+        (fun (h0 : hmem (vprop_of_list tr.r_pre)) ->
+           tr.r_req_eq h0)
+        (fun (h0 : hmem (vprop_of_list tr.r_pre)) x (h1 : hmem (vprop_of_list (tr.r_post x))) ->
+           tr.r_ens_eq h0 x h1))
       f)
 
 inline_for_extraction noextract
@@ -67,13 +51,15 @@ let steel_ghost_of_repr
       (tr : to_repr_t a pre post req ens)
       f
   =
-    (**) steel_of_repr_lem tr;
-    (**) FStar.Classical.forall_intro tr.r_req_eq;
-    (**) FStar.Classical.forall_intro_3 tr.r_ens_eq;
+    (**) tr.r_pre_eq ();
+    (**) FStar.Classical.forall_intro tr.r_post_eq;
+    (**) FStar.Classical.forall_intro_2 reveal_equiv;
     SH.unit_steel_ghost_subcomp_no_frame #a #opened
       _ _ req ens
       (tr.r_pre_eq ()) (fun x -> tr.r_post_eq x)
-      ()
+      (SH.intro_subcomp_no_frame_pre _ _ _ _ _ _
+        (fun h0      -> tr.r_req_eq h0)
+        (fun h0 x h1 -> tr.r_ens_eq h0 x h1))
       (SH.ghost_u f)
 
 inline_for_extraction noextract
@@ -83,16 +69,17 @@ let repr_steel_of_steel_ghost
       ($f  : SH.unit_steel_ghost a opened pre post req ens)
   : repr_steel_t (SH.KGhost opened) a tr.r_pre tr.r_post tr.r_req tr.r_ens
   =
-    (**) steel_of_repr_lem tr;
-    (**) repr_steel_of_steel_lem tr;
-    (**) FStar.Classical.forall_intro tr.r_req_eq;
-    (**) FStar.Classical.forall_intro_3 tr.r_ens_eq;
+    (**) tr.r_pre_eq ();
+    (**) FStar.Classical.forall_intro tr.r_post_eq;
+    (**) FStar.Classical.forall_intro_2 reveal_equiv;
     SH.ghost_f #opened (SH.unit_steel_ghost_subcomp_no_frame
       req ens _ _
       () (fun _ -> ())
       (SH.intro_subcomp_no_frame_pre _ _ _ _ _ _
-        (fun h0 -> tr.r_req_eq (focus_rmem h0 pre))
-        (fun h0 x h1 -> tr.r_ens_eq (focus_rmem h0 pre) x (focus_rmem h1 (post x))))
+        (fun (h0 : hmem (vprop_of_list tr.r_pre)) ->
+           tr.r_req_eq h0)
+        (fun (h0 : hmem (vprop_of_list tr.r_pre)) x (h1 : hmem (vprop_of_list (tr.r_post x))) ->
+           tr.r_ens_eq h0 x h1))
       f)
 
 
@@ -106,14 +93,14 @@ let spec_r_of_find_ro
   = SH.steel_f (fun () ->
       (**) let sl0    = gget_f sro.sro_spc.spc_pre in
       (**) let sl_fr0 = gget_f sro.sro_spc.spc_ro  in
-      (**) steel_intro_vprop_of_list_append_f sro.sro_spc.spc_pre sro.sro_spc.spc_ro;
-      (**) steel_change_perm sro.sro_pre_eq;
+      (**) intro_vpl_append sro.sro_spc.spc_pre sro.sro_spc.spc_ro;
+      (**) change_vpl_perm sro.sro_pre_eq;
       (**) sro.sro_req_eq sl0 sl_fr0;
       let (x : a) = SH.steel_u f ()     in
       (**) let sl1'   = gget_f (post x) in
-      (**) steel_change_perm (sro.sro_post_eq x);
+      (**) change_vpl_perm (sro.sro_post_eq x);
       (**) extract_vars_sym_l (sro.sro_post_eq x) sl1';
-      (**) steel_elim_vprop_of_list_append_f (sro.sro_spc.spc_post x) sro.sro_spc.spc_ro;
+      (**) elim_vpl_append (sro.sro_spc.spc_post x) sro.sro_spc.spc_ro;
       (**) let sl1    = gget_f (sro.sro_spc.spc_post x) in
       (**) let sl_fr1 = gget_f sro.sro_spc.spc_ro       in
       (**) sro.sro_ens_eq sl0 sl_fr0 x sl1 sl_fr1;
@@ -129,14 +116,14 @@ let spec_r_of_find_ro_ghost
   = SH.ghost_f (fun () ->
       (**) let sl0    = gget_f sro.sro_spc.spc_pre in
       (**) let sl_fr0 = gget_f sro.sro_spc.spc_ro  in
-      (**) steel_intro_vprop_of_list_append_f sro.sro_spc.spc_pre sro.sro_spc.spc_ro;
-      (**) steel_change_perm sro.sro_pre_eq;
+      (**) intro_vpl_append sro.sro_spc.spc_pre sro.sro_spc.spc_ro;
+      (**) change_vpl_perm sro.sro_pre_eq;
       (**) sro.sro_req_eq sl0 sl_fr0;
       let (x : a) = SH.ghost_u f ()     in
       (**) let sl1'   = gget_f (post x) in
-      (**) steel_change_perm (sro.sro_post_eq x);
+      (**) change_vpl_perm (sro.sro_post_eq x);
       (**) extract_vars_sym_l (sro.sro_post_eq x) sl1';
-      (**) steel_elim_vprop_of_list_append_f (sro.sro_spc.spc_post x) sro.sro_spc.spc_ro;
+      (**) elim_vpl_append (sro.sro_spc.spc_post x) sro.sro_spc.spc_ro;
       (**) let sl1    = gget_f (sro.sro_spc.spc_post x) in
       (**) let sl_fr1 = gget_f sro.sro_spc.spc_ro       in
       (**) sro.sro_ens_eq sl0 sl_fr0 x sl1 sl_fr1;
